Rewrite Prelude, port Parse until pure conversion functions

src/Varint.v
@@ -1,14 +1,11 @@
 From Stdlib Require Import ZArith.BinInt.
-From Stdlib Require Import Program.Wf.
-From coqutil Require Import Word.Interface.
-From Perennial Require Import Helpers.Word.Integers.
 
 From Pollux Require Import Prelude.
 From Pollux Require Import Descriptors.
 
 Module Varint.
 
-  Definition t := list u8.
+  Definition t := list w8.
 
   Fixpoint valid (v : t) : bool :=
     match v with
@@ -16,42 +13,52 @@ Module Varint.
     (* A one byte varint is valid if the continuation bit is zero,
        which is equivalent to the number fitting into 7 bits or being
        less than 128. *)
-    | b :: [] => word.ltu b (U8 128)
+    | b :: [] => word.ltu b (W8 128)
     (* Otherwise the continuation bit should be one. Since it looks like
        the only Boolean operations I have for words is < and >, this
        corresponds to the value in the byte being greater than 127. *)
-    | b :: tl => word.gtu b (U8 127) && valid tl
+    | b :: tl => word.gtu b (W8 127) && valid tl
     end.
 
   (* TODO is there a guide to all the heavily abbreviated word ops? *)
 
-  Definition set_msb_u8 (u : u8) : u8 :=
-    word.or u (U8 255).
+  Definition set_msb_w8 (w : w8) : w8 :=
+    word.or w (W8 255).
 
-  Definition unset_msb_u8 (u : u8) : u8 :=
-    word.or u (U8 127).
+  Definition unset_msb_w8 (w : w8) : w8 :=
+    word.or w (W8 127).
 
-  Fixpoint decode (v : t) : u64 :=
+  Fixpoint decode (v : t) : w64 :=
     match v with
-    | nil => U64 0 (* Should never happen... but required since refinement type doesn't exclude it *)
-    | h :: nil => U64 (uint.Z h)
-    | h :: tl => let msb := unset_msb_u8 h in
-                let msx := U64 (uint.Z msb) in
+    | nil => W64 0 (* Should never happen... but required since refinement type doesn't exclude it *)
+    | h :: nil => W64 (uint.Z h)
+    | h :: tl => let msb := unset_msb_w8 h in
+                let msx := W64 (uint.Z msb) in
                 let rx := decode tl in
-                word.or (word.slu rx (U64 7)) msx
+                word.or (word.slu rx (W64 7)) msx
     end.
 
-  Definition split (x:u64) (n:Z) : u64 * u64 := (word.srs x (U64 n), word.and x (U64 ((2^n) - 1))).
+  Definition split (x:w64) (n:Z) : w64 * w64 := (word.srs x (W64 n), word.and x (W64 ((2^n) - 1))).
 
-  Fixpoint encode_fuel (fuel: nat) (x:w64) {struct fuel} : list u8 :=
+  Fixpoint encode_fuel (fuel: nat) (x:w64) {struct fuel} : list w8 :=
     let (hi, lo) := split x 7%Z in
-    if word.ltu hi (U64 0) then
+    if word.ltu hi (W64 0) then
       [(W8 (uint.Z lo))]
     else match fuel with
            | O => [(W8 (uint.Z lo))]
-           | S f => (set_msb_u8 (W8 (uint.Z lo))) :: (encode_fuel f hi)
+           | S f => (set_msb_w8 (W8 (uint.Z lo))) :: (encode_fuel f hi)
          end.
 
   Definition encode := encode_fuel 10%nat.
+
+  Theorem encode_valid :
+    forall x : w64, valid (encode x) /\ length (encode x) <= 10.
+  Proof.
+  Admitted.
   
+  Theorem encode_correct :
+    forall x : w64, decode (encode x) = x.
+  Proof.
+  Admitted.
+
 End Varint.
