src/Parse.v
@@ -1,0 +1,43 @@
+From Pollux Require Import Prelude.
+
+From Pollux Require Import Descriptors.
+From Pollux Require Import Varint.
+
+Module Parse.
+
+  Include Descriptors.
+  Infix "%" := Z.modulo (at level 35) : Z_scope.
+  Infix "==" := Z.eqb (at level 35) : Z_scope.
+
+  Definition parity (z : Z) : Z :=
+    if ((z % 2) == 0)%Z then 1 else (-1).
+
+  Definition idn (c : bool) : Z := if c then 1 else 0.
+
+  Definition uint_change_w (w : Width) (v : Z) : Z := v % (2^(unwrap_width w)).
+  Definition int_change_w (w : Width) (v : Z) : Z := let pow2__w := (2^((unwrap_width w) - 1))%Z in
+                                                     (v `mod` pow2__w - pow2__w * idn (( v / pow2__w) % 2 == 1)).
+  Definition sint_change_w (w : Width) (v : Z) : Z := let pow2__w := (2^((unwrap_width w) - 1))%Z in
+                                                      (v `mod` pow2__w - pow2__w * idn (Z.ltb v 0)).
+  Definition uint_int (w : Width) (v : Z) : Z := v - (2^(unwrap_width w)) *
+                                                       (idn (Z.geb v (2^(unwrap_width w - 1))%Z)).
+  Definition int_uint (w : Width) (v : Z) : Z := v + (2^(unwrap_width w)) * (idn (Z.ltb v 0)).
+  Definition uint_sint (w : Width) (v : Z) : Z := parity v * (v / 2) - (v % 2).
+  Definition sint_uint (w : Width) (v : Z) : Z := 2 * (Z.abs v) - idn (Z.ltb v 0).
+  Definition int_sint (w : Width) (v : Z) : Z := if Z.geb v 0 then
+                                                   parity v * (v / 2) - (v % 2)
+                                                 else
+                                                   parity v * (v + (2^(unwrap_width w - 1)) - (v / 2)).
+  Definition sint_int (w : Width) (v : Z) : Z := if Z.leb (- 2^(unwrap_width w - 2)) v &&
+                                                      Z.leb v (2^(unwrap_width w - 2)) then
+                                                   2 * (Z.abs v) - idn (Z.ltb v 0)
+                                                 else
+                                                   2 * (Z.abs v) - (2^(unwrap_width w)) - idn (Z.ltb v 0).
+
+    (* NOTE: Compared to the F* version, these functions no longer have type-level assurances
+       that the resulting integer is in-bounds for the given width. Now, the F* functions only
+       had this assurance, so the formula could still be wrong, which is why there were / are
+       tested against the official protobuf implementation.
+     *)
+  
+End Parse.
